cp

pulse/lib/steel/pulse/Pulse.Checker.Auto.Util.fsti
@@ -142,7 +142,7 @@ type prover_state (preamble:preamble) = {
 }
 
 let pst_extends (#preamble:_) (p1 p2:prover_state preamble) =
-  p2.ss `Psubst.subst_extends` p1.ss
+  p1.ss `Psubst.subst_extends` p2.ss
 
 type prover_t =
   #preamble:_ ->
@@ -265,7 +265,7 @@ let prove_precondition (#g:env) (#ctxt:term) (ctxt_typing:vprop_typing g ctxt)
 let intro_exists_sub_prover_state (#preamble:_) (p:prover_state preamble)
   (u:universe) (b:binder) (body:vprop)
   (exists_typing:tot_typing (pst_env preamble.uvs p.ss) (Tm_ExistsSL u b body) Tm_VProp)
-  : v:var &
+  : x:var { ~ (x `Set.mem` (Set.union (dom preamble.g0) (dom preamble.uvs)))} &
     preamble:_ &
     prover_state preamble =
   
@@ -361,1011 +361,216 @@ let intro_exists_sub_prover_state (#preamble:_) (p:prover_state preamble)
       c_pre_inv; solved_goals_closed = () } |)
 
 
-#push-options "--z3rlimit_factor 10 --fuel 2 --ifuel 2"
+#push-options "--fuel 2 --ifuel 2 --query_stats --using_facts_from '* -FStar.Reflection -Steel'"
 let intro_exists_step (#preamble:_) (p:prover_state preamble)
-  (u:universe) (b:binder) (body:vprop) (unmatched':list vprop)
-  (_:squash (p.unmatched == (Tm_ExistsSL u b body) :: unmatched'))
+  (u:universe) (b:binder) (body:vprop) (unsolved_goals':list vprop)
+  (_:squash (p.unsolved_goals == (Tm_ExistsSL u b body) :: unsolved_goals'))
   (prover:prover_t)
-  : T.Tac (option (p':prover_state preamble { p'.uvs `env_extends` p.uvs })) =
+  : T.Tac (option (p':prover_state preamble { p' `pst_extends` p })) =
   
-
-  let (| x, sub_prover_preamble, sub_prover_state |) = intro_exists_sub_prover_state 
-    p u b body (magic ()) in
-
-  let sub_prover_state = prover sub_prover_state in
-
-  match sub_prover_state with
+  let g0 = preamble.g0 in
+  let (| x, s_preamble, sp |) = intro_exists_sub_prover_state 
+    p u b body
+    (magic ())  // typing of Tm_ExistsSL, should come from the typing of unmatched goals
+  in
+  let sp = prover sp in
+  match sp with
   | None -> None
-  | Some sub_prover_state ->
-    let sub_steps_typing
-      : st_typing (push_env preamble.g0 sub_prover_state.uvs)
-                  sub_prover_state.steps
-                  (ghost_comp (list_as_vprop p.remaining)
-                              (Tm_Star (list_as_vprop sub_prover_state.remaining)
-                                       (subst_term sub_prover_state.matched sub_prover_state.ss))) =
-      sub_prover_state.steps_typing in
+  | Some sp ->
+    // The following code to finish a terminal prover state is common
+    //   with the top-level prover, could be factored out
+    if x `Set.mem` Psubst.dom sp.ss
+    then begin
+      let c_pre_inv:
+        vprop_equiv (pst_env s_preamble.uvs sp.ss)
+                    (Psubst.subst_term sp.ss (comp_pre s_preamble.c))
+                    (Tm_Star (list_as_vprop []) sp.solved_goals) = sp.c_pre_inv in
+      // normalize list_as_vprop []
+      let c_pre_inv:
+        vprop_equiv (pst_env s_preamble.uvs sp.ss)
+                    (Psubst.subst_term sp.ss (comp_pre s_preamble.c))
+                    sp.solved_goals = magic () in
+      let remaining_ctxt = list_as_vprop sp.remaining_ctxt in
+      let steps_typing:
+        st_typing (pst_env s_preamble.uvs sp.ss) sp.steps
+          (ghost_comp s_preamble.ctxt (Tm_Star remaining_ctxt sp.solved_goals)) = sp.steps_typing in
+      // replace pst.solved_goals with equivalent (Psubst.subst_term pst.ss (comp_pre preamble.c))
+      //   from c_pre_inv
+      // note that all these postconditions are ln
+      let steps_typing:
+        st_typing (pst_env s_preamble.uvs sp.ss) sp.steps
+          (ghost_comp s_preamble.ctxt
+                      (Tm_Star remaining_ctxt
+                               (Psubst.subst_term sp.ss (comp_pre s_preamble.c)))) = magic () in
+      let t_typing:
+        st_typing (pst_env s_preamble.uvs sp.ss)
+                  (Psubst.subst_st_term sp.ss s_preamble.t)
+                  (Psubst.subst_comp sp.ss s_preamble.c) = sp.t_typing in
+      assert (comp_pre (Psubst.subst_comp sp.ss s_preamble.c) ==
+              Psubst.subst_term sp.ss (comp_pre s_preamble.c));
+      // NT substs are invariant under shifting
+      assume (shift_subst (Psubst.as_subst sp.ss) == Psubst.as_subst sp.ss);
+      assert (comp_post (Psubst.subst_comp sp.ss s_preamble.c) ==
+              Psubst.subst_term sp.ss (Tm_ExistsSL u b body));
+      // bind steps_typing and t_typing
+      // what's left is remaining ctxt and exists vprop
+      let t : st_term = magic () in
+      let t_typing:
+        st_typing (pst_env s_preamble.uvs sp.ss)
+                  t
+                  (ghost_comp
+                     s_preamble.ctxt
+                     (Tm_Star remaining_ctxt (Psubst.subst_term sp.ss (Tm_ExistsSL u b body))))
+        = magic () in
+
+      // now we get back to the original prover we got,
+      //   and have to find a way to combine the two
     
-    let sub_veq : vprop_equiv (push_env preamble.g0 sub_prover_state.uvs)
-                              (comp_pre sub_prover_preamble.c)
-                              (Tm_Star (list_as_vprop []) sub_prover_state.matched) =
-      sub_prover_state.veq in
-    // normalize list_as_vprop []
-    let sub_veq : vprop_equiv (push_env preamble.g0 sub_prover_state.uvs)
-                              (comp_pre sub_prover_preamble.c)
-                              sub_prover_state.matched = magic () in
-    // PARTIAL SUBSTITUTION STEP, APPLY THE SUBSTITUTION BUT KEEP ENV SAME
-    assume (push_env preamble.g0 sub_prover_state.uvs ==
-            push_env preamble.g0 (push_env sub_prover_state.uvs (mk_env (fstar_env preamble.g0))));
-    assume (subst_env (mk_env (fstar_env preamble.g0)) sub_prover_state.ss == mk_env (fstar_env preamble.g0));
-    let sub_veq : vprop_equiv (push_env preamble.g0 (push_env sub_prover_state.uvs (mk_env (fstar_env preamble.g0))))
-                              (comp_pre sub_prover_preamble.c)
-                              sub_prover_state.matched = coerce_eq sub_veq () in
-    let sub_veq : vprop_equiv (push_env preamble.g0 (push_env sub_prover_state.uvs (subst_env (mk_env (fstar_env preamble.g0)) sub_prover_state.ss)))
-                              (subst_term (comp_pre sub_prover_preamble.c) sub_prover_state.ss)
-                              (subst_term sub_prover_state.matched sub_prover_state.ss) =
-      veq_subst_partial
-        preamble.g0
-        sub_prover_state.uvs
-        (mk_env (fstar_env preamble.g0))
-        sub_veq
-        sub_prover_state.ss in
-    let sub_veq : vprop_equiv (push_env preamble.g0 sub_prover_state.uvs)
-                              (subst_term (comp_pre sub_prover_preamble.c) sub_prover_state.ss)
-                              (subst_term sub_prover_state.matched sub_prover_state.ss) =
-      coerce_eq sub_veq () in
+      let uvs = psubst_env (filter_ss preamble.uvs p.ss) p.ss in
+      let uvs = push_binding uvs x b.binder_ty in
 
-    // use sub_veq with sub_steps_typing
-    let sub_steps_typing
-      : st_typing (push_env preamble.g0 sub_prover_state.uvs)
-                  sub_prover_state.steps
-                  (ghost_comp (list_as_vprop p.remaining)
-                              (Tm_Star (list_as_vprop sub_prover_state.remaining)
-                                       (subst_term (comp_pre sub_prover_preamble.c) sub_prover_state.ss))) =
-      magic () in
 
-    let t_typing
-      : st_typing (push_env preamble.g0 sub_prover_state.uvs)
-                  sub_prover_preamble.t
-                  sub_prover_preamble.c = sub_prover_state.t_typing in
+      // target : pst_env preamble.uvs (ss + p.ss)
+      assume (~ (x `Set.mem` dom g0));
+      assume (freevars (Psubst.lookup sp.ss x) `Set.subset` dom g0);
+      assume (Set.subset (Psubst.dom (Psubst.singleton g0 x (Psubst.lookup sp.ss x))) (Psubst.dom sp.ss));
+      let sp_ss = Psubst.diff sp.ss (Psubst.singleton g0 x (Psubst.lookup sp.ss x)) in
+      assume (Set.disjoint (Psubst.dom p.ss) (Psubst.dom sp_ss));  // this takes time ...
+      assume (equal (pst_env s_preamble.uvs sp.ss)
+                    (pst_env preamble.uvs (Psubst.push p.ss sp_ss)));
+      // calc (equal) {
+      //   pst_env s_preamble.uvs sp.ss;
+      //      (equal) { }
+      //   pst_env (push_binding (psubst_env (filter_ss preamble.uvs p.ss) p.ss) x b.binder_ty) sp.ss;
+      //      (equal) { assume (Psubst.subst_term p.ss b.binder_ty == b.binder_ty) }  // b.binder_ty freevars should be disjoint from p.ss
+      //   pst_env (push_binding (psubst_env (filter_ss preamble.uvs p.ss) p.ss) x (Psubst.subst_term p.ss b.binder_ty)) sp.ss;
+      //      (equal) { assume (push_binding (psubst_env (filter_ss preamble.uvs p.ss) p.ss) x (Psubst.subst_term p.ss b.binder_ty) ==
+      //                        psubst_env (push_binding (filter_ss preamble.uvs p.ss) x b.binder_ty) p.ss) }
+      //   pst_env (psubst_env (push_binding (filter_ss preamble.uvs p.ss) x b.binder_ty) p.ss) sp.ss;
+      //      (equal) { assume (push_binding (filter_ss preamble.uvs p.ss) x b.binder_ty ==
+      //                        filter_ss (push_binding preamble.uvs x b.binder_ty) p.ss) }  // p.ss does not have x
+      //   pst_env (psubst_env (filter_ss (push_binding preamble.uvs x b.binder_ty) p.ss) p.ss) sp.ss;
+      //      (equal) { }
+      //   push_env g0 (psubst_env (filter_ss (psubst_env (filter_ss (push_binding preamble.uvs x b.binder_ty) p.ss) p.ss) sp.ss) sp.ss);
+      //      (equal) { admit () }  // some commutations of filter and push, and then pushing substs,
+      //                            // with the fact that x is in sp.ss, we checked it above
+      //   pst_env preamble.uvs (Psubst.push p.ss sp.ss);
+      // };
 
-    // similar manipulations and PARTIAL SUBSTITUTIONS LEMMA ON st_typing, to get:
-    let t_typing
-      : st_typing (push_env preamble.g0 sub_prover_state.uvs)
-                  (subst_st_term sub_prover_preamble.t sub_prover_state.ss)
-                  (subst_comp sub_prover_preamble.c sub_prover_state.ss) = magic () in
+      let ss_new = Psubst.push p.ss sp_ss in
+      let uvs = psubst_env (filter_ss preamble.uvs p.ss) p.ss in
+      assume (well_typed_ss uvs sp_ss);
+      assume (push_env g0 (psubst_env (filter_ss uvs sp_ss) sp_ss) ==
+              pst_env preamble.uvs ss_new);  // may be we can make a single combinator for filter and push,
+                                             // and prove subst push lemma for it
 
-    assert (sub_prover_preamble.c ==
-            ghost_comp (comp_pre sub_prover_preamble.c)
-                       (Tm_ExistsSL u b body));
-    // NT substitutions are invariant under shifting
-    assume (shift_subst sub_prover_state.ss == sub_prover_state.ss);
-    assert (subst_comp sub_prover_preamble.c sub_prover_state.ss ==
-            ghost_comp (subst_term (comp_pre sub_prover_preamble.c) sub_prover_state.ss)
-                       (subst_term (Tm_ExistsSL u b body) sub_prover_state.ss));
-
-    // we have:
-    // g0, uvs |- { p.remaining } sub.steps { sub.remaining * ss (pre subpreamble.c)}
-    // and
-    // g0, uvs |- { ss (pre subpreamble.c) } ss sub.t { ss (Tm_ExistsSL u b body) }
-    // we can bind these to get:
-    //
-    // g0, uvs |- { p.remaining } bind { sub.remaining * ss (Tm_ExistsSL u b body) }
-    let sub_steps : st_term = magic () in
-    let sub_steps_typing
-      : st_typing (push_env preamble.g0 sub_prover_state.uvs)
-                  sub_steps
-                  (ghost_comp (list_as_vprop p.remaining)
-                              (Tm_Star (list_as_vprop sub_prover_state.remaining)
-                                       (subst_term (Tm_ExistsSL u b body) sub_prover_state.ss))) = magic () in
-
-    // now stitch these steps in the original prover we got
-
-    let psteps_typing
-      : st_typing (push_env preamble.g0 p.uvs)
+      let pt_typing:
+        st_typing (pst_env preamble.uvs p.ss)
                   p.steps
-                  (ghost_comp preamble.ctxt
-                              (Tm_Star (list_as_vprop p.remaining) (subst_term p.matched p.ss))) = p.steps_typing in
+                  (ghost_comp
+                     preamble.ctxt
+                     (Tm_Star (list_as_vprop p.remaining_ctxt) p.solved_goals)) = p.steps_typing in
 
-    ss_extends_subst preamble.g0 p.uvs sub_prover_state.uvs p.ss sub_prover_state.ss p.matched;
-    assert (subst_term p.matched p.ss == subst_term p.matched sub_prover_state.ss);
-    
-    let psteps_typing
-      : st_typing (push_env preamble.g0 p.uvs)
-                  p.steps
-                  (ghost_comp preamble.ctxt
-                              (Tm_Star (list_as_vprop p.remaining) (subst_term p.matched sub_prover_state.ss))) = p.steps_typing in
+      let (| _, pt_typing |) = apply_partial_subs uvs sp_ss pt_typing in
+      let pt_typing:
+        st_typing (pst_env preamble.uvs ss_new)
+                  (Psubst.subst_st_term sp_ss p.steps)
+                  (Psubst.subst_comp sp_ss (ghost_comp preamble.ctxt (Tm_Star (list_as_vprop p.remaining_ctxt) p.solved_goals))) =
+        coerce_eq pt_typing () in
+      // p.solved goals is closed in g0, and p.remaining_ctxt is well typed in g0
+      assume (Psubst.subst_comp sp_ss (ghost_comp preamble.ctxt (Tm_Star (list_as_vprop p.remaining_ctxt) p.solved_goals)) ==
+              ghost_comp preamble.ctxt (Tm_Star (list_as_vprop p.remaining_ctxt) p.solved_goals));
+      let pt_typing:
+        st_typing (pst_env preamble.uvs ss_new)
+                  (Psubst.subst_st_term sp_ss p.steps)
+                  (ghost_comp preamble.ctxt (Tm_Star s_preamble.ctxt p.solved_goals)) = coerce_eq pt_typing () in
+      // recall t_typing from above, from sub prover state
+      let t_typing:
+        st_typing (pst_env preamble.uvs ss_new)
+                  t
+                  (ghost_comp
+                     s_preamble.ctxt
+                     (Tm_Star remaining_ctxt (Psubst.subst_term sp.ss (Tm_ExistsSL u b body))))
+        = coerce_eq t_typing () in
 
-    assert (sub_prover_state.uvs `env_extends` p.uvs);
-    // weakening of gamma
-    let psteps_typing
-      : st_typing (push_env preamble.g0 sub_prover_state.uvs)
-                  p.steps
-                  (ghost_comp preamble.ctxt
-                              (Tm_Star (list_as_vprop p.remaining) (subst_term p.matched sub_prover_state.ss))) =
-        magic () in
-
-    // we have:
-    // g0, uvs |- { preamble.ctxt } p.steps { p.remaining * sub_prover_state.ss p.matched }
-    // and
-    // g0, uvs |- { p.remaining } sub_steps { sub_prover_state.remaining * sub_prover_state.ss (Tm_ExistsSL u b body) }
-    //
-    // we can bind these to get:
-    //
-    // g0, uvs |- { preamble.ctxt } bind { sub_prover_state.remaining * sub_prover_state.ss (exists::p.matched) }
-    let steps : st_term = magic () in
-    let steps_typing
-      : st_typing (push_env preamble.g0 sub_prover_state.uvs)
+      // bind pt_typing and t_typing
+      let steps : st_term = magic () in
+      let steps_typing:
+        st_typing (pst_env preamble.uvs ss_new)
                   steps
-                  (ghost_comp preamble.ctxt
-                              (Tm_Star (list_as_vprop sub_prover_state.remaining)
-                                       (subst_term (Tm_Star (Tm_ExistsSL u b body) p.matched) sub_prover_state.ss))) =
-      magic () in
-
-    let uvs = sub_prover_state.uvs in
-    let ss = sub_prover_state.ss in
-    let matched = Tm_Star (Tm_ExistsSL u b body) p.matched in
-    let unmatched = unmatched' in
-    let remaining = sub_prover_state.remaining in
-
-    assume ((push_env preamble.g0 uvs) `env_extends` push_env preamble.g0 p.uvs);
-
-    // weakening of gamma
-    let t_typing : st_typing (push_env preamble.g0 uvs) preamble.t preamble.c = magic () in
-
-    // derive from p.unmatched typing and weakening of gamma
-    let unmatched_typing
-      : tot_typing (push_env preamble.g0 uvs) (list_as_vprop unmatched) Tm_VProp = magic () in
-
-    let remaining_typing
-      : tot_typing preamble.g0 (list_as_vprop remaining) Tm_VProp = sub_prover_state.remaining_typing in
-
-    let steps_typing
-      : st_typing (push_env preamble.g0 uvs)
-                  steps
-                  (ghost_comp preamble.ctxt
-                              (Tm_Star (list_as_vprop remaining)
-                                       (subst_term matched ss))) = steps_typing in
-
-    // move Tm_ExistsSL from unmatched to matched and weaken gamma
-    let veq : vprop_equiv (push_env preamble.g0 uvs)
-                          (comp_pre preamble.c)
-                          (Tm_Star (list_as_vprop unmatched) matched) = magic () in
-
-    // TODO: THIS NEEDS TO BE A RUNTIME CHECK THAT WE CLOSED EXISTS
-    assume (freevars (subst_term (Tm_ExistsSL u b body) sub_prover_state.ss) `Set.subset` dom preamble.g0);
-
-    Some ({
-      uvs; ss;
-      matched; unmatched; remaining; steps;
-      t_typing; unmatched_typing; remaining_typing; steps_typing; veq; ss_closes_matched_uvs = ()
-    })
-
-
-
-
-// let vprop_typing g v = tot_typing g v Tm_VProp
-
-// let ghost_comp pre post = 
-//   C_STGhost Tm_EmpInames { u=u_zero; res=tm_unit; pre; post }
-
-// open Pulse.Checker.VPropEquiv
-
-
-// ///// Sketch of the new prover /////
-
-// val dom_env (g:env) : Set.set var
-// type typ = term
-
-// // uvars with their types
-// type uvs_t = Map.t var typ
-
-// type substitution = Map.t var term
-
-// val apply_ss (s:substitution) (t:term) : term
-// val apply_ss_st (s:substitution) (t:st_term) : st_term
-// val apply_c (s:substitution) (c:comp) : comp
-
-// let uvars (t:term) (uvs:uvs_t) : Set.set var =
-//   Set.intersect (freevars t) (Map.domain uvs)
-// let uvars_st (t:st_term) (uvs:uvs_t) : Set.set var =
-//   Set.intersect (freevars_st t) (Map.domain uvs)
-
-// val env_contains (g:env) (x:var) (t:typ) : prop
-
-// let set_difference (#a:eqtype) (s1 s2:Set.set a) =
-//   Set.intersect s1 (Set.complement s2)
-
-
-// //
-// // In the prover state we maintain two environments,
-// //   g0: the environment when we enter the prover, it doesn't have any uvars
-// //    g: the current environment, may have names which are used as uvars
-// //
-
-// // TODO: we need to add a notion of well-typed env
-// // and maintain that
-// let uvs_invariant (g0 g:env) (uvs:uvs_t) : prop =
-//   g `env_extends` g0 /\
-//   Set.equal (set_difference (dom_env g) (dom_env g0)) (Map.domain uvs) /\
-//   (forall (x:var). Map.contains uvs x ==>
-//                    env_contains g x (Map.sel uvs x))
-
-// //
-// // The preamble remains fixed as prover state is transformed by steps
-// //
-// noeq
-// type prover_state_preamble = {
-//   // top-level entry env, no uvars
-//   // when we enter the prover
-//   // env into which we will elaborate the proof steps
-//   // also the env in which the ctxt is well-typed
-//   // initial_env
-//   g0:env;
-//   // current_env (g0 + uvars)
-//   g:env;
-//   // initial context
-//   ctxt:vprop;
-//   // ctxt is well-typed in g0
-//   // we never introduce uvars in the ctxt
-//   // initial_ctxt_typing
-//   ctxt_typing:vprop_typing g0 ctxt;
-//   // term whose precondition is the goal
-//   t:st_term;
-//   // comp for t
-//   c:comp_st;
-//   // t and c however may contain uvars
-//   t_typing:st_typing g t c;
-
-//   // set of uvars and their types that we have introduced so far
-//   uvs:uvs_t;
-//   // uvars are well-typed in g
-//   uvs_props:squash (uvs_invariant g0 g uvs);
-// }
-
-// //
-// // TODO:
-// //   would like to have this: freevars t in g, and no uvars in t, then freevars t in g0
-// //
-
-// //
-// // Solutions to uvars are closed in g0 --- no uvars in them
-// //
-
-// // TODO: this doesn't allow for dependent uvars,
-// //   type of a uvar depending on another uvar
-// // We need to close the telescope when stating this
-// // Perhaps better to keep uvars and substs also as env,
-// //   so that we get well-formedness for free
-// let well_typed_substitution (g0:env) (uvs:uvs_t) (ss:substitution) : prop =
-//   dom_env g0 `Set.disjoint` Map.domain uvs /\
-//   (forall (x:var). Map.contains ss x ==>
-//                    (Map.contains uvs x /\
-//                     tot_typing g0 (Map.sel ss x) (Map.sel uvs x)))
-
-// noeq
-// type prover_state (preamble:prover_state_preamble) = {
-//   // things in cpre that we have solved
-//   // rename to solved_conjuncts
-//   matched:term;
-//   // remaining things in cpre
-//   // goals
-//   unmatched:list term;
-//   // context remaining that we can match from
-//   // remaining_ctxt
-//   remaining:list term;
-//   // the proof steps we have accumulated so far
-//   // proof_steps
-//   steps:st_term;
-
-//   // uvars -> terms
-//   ss:substitution;
-
-//   // remaining is well-typed in g0
-//   // remaining_ctxt_typing
-//   remaining_typing:vprop_typing preamble.g0 (list_as_vprop remaining);
-
-//   // goals_typing
-//   unmatched_typing:vprop_typing preamble.g (list_as_vprop unmatched);
-
-//   // steps are well-typed in g0
-//   // proof_steps_typing
-//   steps_typing:st_typing preamble.g0 steps
-//     (ghost_comp
-//        preamble.ctxt
-//        (Tm_Star (list_as_vprop remaining) (apply_ss ss matched)));
-
-//   // we haven't dropped any of the initial goals
-//   // inductive invariant to relate solved goals and remaining goals
-//   veq:vprop_equiv preamble.g (comp_pre preamble.c)
-//                              (Tm_Star (list_as_vprop unmatched) matched);
-
-//   props:squash (
-//     well_typed_substitution preamble.g0 preamble.uvs ss /\
-//     // whatever has been matched, must be closed w.r.t. uvars
-//     uvars matched preamble.uvs `Set.subset` Map.domain ss
-//   );
-// }
-
-// let ss_extends (ss1 ss2:substitution) : prop =
-//   forall (x:var). (Map.contains ss2 x ==> (Map.contains ss1 x /\
-//                                            Map.sel ss1 x == Map.sel ss2 x))
-
-// val apply_ss_uvars (g0:env) (uvs:uvs_t) (ss:substitution) (t:term)
-//   : Lemma
-//       (requires well_typed_substitution g0 uvs ss)
-//       (ensures uvars (apply_ss ss t) uvs ==
-//                set_difference (uvars t uvs) (Map.domain ss))
-
-// val apply_ss_st_uvars (g0:_) (uvs:_) (ss:substitution) (t:st_term)
-//   : Lemma
-//       (requires well_typed_substitution g0 uvs ss)
-//       (ensures uvars_st (apply_ss_st ss t) uvs ==
-//                set_difference (uvars_st t uvs) (Map.domain ss))
-
-// val apply_ss_star (ss:substitution) (p1 p2:vprop)
-//   : Lemma (apply_ss ss (Tm_Star p1 p2) == apply_ss ss p1 `Tm_Star` apply_ss ss p2)
-
-// val extends_apply (g0:_) (uvs:_) (ss1 ss2:substitution) (t:term)
-//   : Lemma
-//       (requires
-//          well_typed_substitution g0 uvs ss1 /\
-//          well_typed_substitution g0 uvs ss2 /\
-//          ss1 `ss_extends` ss2 /\
-//          uvars t uvs `Set.subset` Map.domain ss2)
-//       (ensures apply_ss ss1 t == apply_ss ss2 t)
-
-// val extends_apply_st (g0:_) (uvs:_) (ss1 ss2:substitution) (t:st_term)
-//   : Lemma
-//       (requires
-//          well_typed_substitution g0 uvs ss1 /\
-//          well_typed_substitution g0 uvs ss2 /\
-//          ss1 `ss_extends` ss2 /\
-//          uvars_st t uvs `Set.subset` Map.domain ss2)
-//       (ensures apply_ss_st ss1 t == apply_ss_st ss2 t)
-
-
-// val typing_ss (g0:_) (uvs:_) (#g:env) (#t:st_term) (#c:comp) (t_typing:st_typing g t c) (ss:substitution)
-//   : Pure (st_typing g (apply_ss_st ss t) (apply_c ss c))
-//          (requires
-//             uvs_invariant g0 g uvs /\
-//             well_typed_substitution g0 uvs ss)
-//          (ensures fun _ -> True)
-
-// val veq_ss (g0:_) (uvs:_) (#g:env) (#p1 #p2:vprop) (veq:vprop_equiv g p1 p2) (ss:substitution)
-//   : Pure (vprop_equiv g (apply_ss ss p1) (apply_ss ss p2))
-//          (requires
-//             uvs_invariant g0 g uvs /\
-//             well_typed_substitution g0 uvs ss)
-//          (ensures fun _ -> True)
-
-// val veq_weakening (#g:_) (#p1 #p2:_) (veq:vprop_equiv g p1 p2) (g':env { env_extends g' g })
-//   : vprop_equiv g' p1 p2
-
-// val st_typing_strengthening (#g:_) (#t:st_term) (#c:comp_st) (t_typing:st_typing g t c)
-//   (g':env { env_extends g g' })
-//   : Pure (st_typing g' t c)
-//          (requires
-//             freevars_st t `Set.subset` dom_env g' /\
-//             freevars_comp c `Set.subset` dom_env g')
-//          (ensures fun _ -> True)
-
-// val tot_typing_strengthening (#g:_) (#t:term) (#ty:term) (t_typing:tot_typing g t ty)
-//   (g':env { env_extends g g' })
-//   : Pure (tot_typing g' t ty)
-//          (requires
-//             freevars t `Set.subset` dom_env g' /\
-//             freevars ty `Set.subset` dom_env g')
-//          (ensures fun _ -> True)
-
-// val veq_strengthening (#g:_) (#p1 #p2:_) (veq:vprop_equiv g p1 p2)
-//   (g':env { env_extends g g' })
-//   : Pure (vprop_equiv g' p1 p2)
-//          (requires
-//             freevars p1 `Set.subset` dom_env g' /\
-//             freevars p2 `Set.subset` dom_env g')
-//          (ensures fun _ -> True)
-
-// let with_pre_post (c:comp_st) (pre:vprop) (post:vprop) : comp_st =
-//   match c with
-//   | C_ST s
-//   | C_STGhost _ s
-//   | C_STAtomic _ s -> with_st_comp c { s with pre; post }
-
-// val pre_post_equiv (#g:env) (#t:st_term) (#c:comp_st {ln (comp_post c)})
-//   (d:st_typing g t c)
-//   (#pre:vprop) (_:vprop_equiv g (comp_pre c) pre)
-//   (#post:vprop) (_:vprop_equiv g (comp_post c) post)
-//   : c':comp_st { c' == with_pre_post c pre post } &
-//     st_typing g t c'
-
-// type prover_t =
-//   #(preamble:_) ->
-//   p:prover_state preamble ->
-//   T.Tac (option (p':prover_state preamble { p'.unmatched == [] /\
-//                                             p'.ss `ss_extends` p.ss }))
-
-// type prover_step =
-//   #(preamble:_) ->
-//   p:prover_state preamble ->
-//   prover:prover_t ->
-//   T.Tac (option (p':prover_state preamble { p'.ss `ss_extends` p.ss }))
-
-
-// let idem_steps (g:env) (ctxt:vprop)
-//   : t:st_term { freevars_st t == Set.empty } &
-//     st_typing g t (ghost_comp ctxt (Tm_Star (list_as_vprop (vprop_as_list ctxt))
-//                                             Tm_Emp)) = magic ()
-
-// val empty_uvs : uvs:uvs_t { Map.domain uvs == Set.empty }
-// val empty_ss : ss:substitution { Map.domain ss == Set.empty }
-
-
-// let prove_precondition (#g:env) (#ctxt:term) (ctxt_typing:tot_typing g ctxt Tm_VProp)
-//   (#t:st_term) (#c:comp_st) (t_typing:st_typing g t c)
-//   (prover:prover_t)
-//   : T.Tac (option (t:st_term &
-//                    c:comp_st { comp_pre c == ctxt } &
-//                    st_typing g t c)) =
-  
-//   assume (g `env_extends` g);
-//   let preamble = {
-//     g0 = g;
-//     g;
-//     ctxt;
-//     ctxt_typing;
-//     t;
-//     c;
-//     t_typing;
-
-//     uvs = empty_uvs;
-//     uvs_props = ()
-//   } in
-
-//   let (| steps, steps_typing |) = idem_steps g ctxt in
-
-//   let matched = Tm_Emp in
-//   let unmatched = vprop_as_list (comp_pre c) in
-//   let remaining = vprop_as_list ctxt in
-//   let steps = steps in
-//   let ss = empty_ss in
-
-//   assume (apply_ss ss matched == Tm_Emp);
-//   let steps_typing : st_typing preamble.g steps
-//     (ghost_comp preamble.ctxt (Tm_Star (list_as_vprop remaining) (apply_ss ss matched))) = steps_typing in
-
-//   let veq : vprop_equiv preamble.g (comp_pre preamble.c)
-//                                    (Tm_Star (list_as_vprop unmatched) matched) = magic () in
-
-//   let p = {
-//     matched;
-//     unmatched;
-//     remaining;
-//     steps;
-//     ss;
-//     remaining_typing = ctxt_typing;
-//     unmatched_typing = magic ();  // get it from inversion of t_typing
-//     steps_typing;
-//     veq;
-//     props = ();
-//   } in
-
-//   let popt = prover p in
-//   match popt with
-//   | Some p' ->
-//     let steps_typing : st_typing g p'.steps
-//       (ghost_comp ctxt (Tm_Star (list_as_vprop p'.remaining)
-//                                 (apply_ss p'.ss p'.matched))) = p'.steps_typing in
-//     assert (Set.equal (Map.domain p'.ss) Set.empty);
-//     // since substitution is empty
-//     assume (apply_ss p'.ss p'.matched == p'.matched);
-//     let steps_typing : st_typing g p'.steps
-//       (ghost_comp ctxt (Tm_Star (list_as_vprop p'.remaining) p'.matched)) = steps_typing in
-
-//     let veq : vprop_equiv g (comp_pre c)
-//                             (Tm_Star (list_as_vprop []) p'.matched) = p'.veq in
-//     // replacing list_as_vprop [] with Tm_Emp and then normalizing star
-//     let veq : vprop_equiv g (comp_pre c) p'.matched = magic () in
-
-//     // use veq with steps_typing
-//     let steps_typing : st_typing g p'.steps
-//       (ghost_comp ctxt (Tm_Star (list_as_vprop p'.remaining) (comp_pre c))) = magic () in
-
-//     // we can now bind p'.steps with c
-
-//     admit ()
-//   | None -> None
-
-// val try_match (g0:_) (uvs:_)
-//   (unm:vprop)
-//   (rem:vprop)
-//   (ss:substitution { well_typed_substitution g0 uvs ss })
-//   : T.Tac (option (ss':substitution { well_typed_substitution g0 uvs ss' /\
-//                                       ss' `ss_extends` ss /\
-//                                       uvars unm uvs `Set.subset` Map.domain ss' } &
-//                    vprop_equiv g0 (apply_ss ss' unm) rem))
-
-
-// let coerce_eq (#a #b:Type) (x:a) (_:squash (a == b)) : y:b { y === x } = x
-
-// let match_step (#preamble:_) (p:prover_state preamble)
-//   (unm:vprop)
-//   (unmatched':list vprop)
-//   (rem:vprop)
-//   (remaining':list vprop)
-//   (veq_unm:vprop_equiv preamble.g (list_as_vprop p.unmatched) (Tm_Star unm (list_as_vprop unmatched')))
-//   (veq_rem:vprop_equiv preamble.g (list_as_vprop p.remaining) (Tm_Star rem (list_as_vprop remaining')))
-
-//   : T.Tac (option (p':prover_state preamble { p'.ss `ss_extends` p.ss })) =
-
-//   let ropt = try_match preamble.g0 preamble.uvs unm rem p.ss in
-//   match ropt with
-//   | Some (| ss', veq_unm_rem |) ->
-//     let matched = Tm_Star unm p.matched in
-//     let unmatched = unmatched' in
-//     let remaining = remaining' in
-
-//     let ss = ss' in
-
-//     ///// restore p.steps_typing /////
-//     extends_apply preamble.g0 preamble.uvs ss p.ss p.matched;
-//     let steps_typing : st_typing preamble.g0 p.steps
-//       (ghost_comp preamble.ctxt
-//          (Tm_Star (list_as_vprop p.remaining) (apply_ss ss p.matched))) =
-//       coerce_eq p.steps_typing () in
-//     // some star rearrangement
-//     let veq: vprop_equiv preamble.g0
-//       (Tm_Star (list_as_vprop p.remaining) (apply_ss ss p.matched))
-//       (Tm_Star (list_as_vprop remaining) (Tm_Star rem (apply_ss ss p.matched))) = magic () in
-//     let veq_unm_rem : vprop_equiv preamble.g0 (apply_ss ss unm) rem =
-//       veq_unm_rem in
-//     let veq : vprop_equiv preamble.g0
-//       (Tm_Star (list_as_vprop p.remaining) (apply_ss ss p.matched))
-//       (Tm_Star (list_as_vprop remaining) (Tm_Star (apply_ss ss unm) (apply_ss ss p.matched))) =
-//       magic () in
-//     apply_ss_star ss unm p.matched;
-//     let veq : vprop_equiv preamble.g0
-//       (Tm_Star (list_as_vprop p.remaining) (apply_ss ss p.matched))
-//       (Tm_Star (list_as_vprop remaining) (apply_ss ss (Tm_Star unm p.matched))) = veq in
-//     let veq_pre : vprop_equiv preamble.g0 preamble.ctxt preamble.ctxt = magic () in
-//     assume (ln (Tm_Star (list_as_vprop p.remaining) (apply_ss ss p.matched)));
-//     let (| _, steps_typing |) : x:_ & st_typing preamble.g0 p.steps
-//       (ghost_comp preamble.ctxt
-//          (Tm_Star (list_as_vprop remaining) (apply_ss ss matched))) =
-//       pre_post_equiv steps_typing veq_pre veq in
-//     /////
-
-//     ///// restore p.veq /////
-//     let veq : vprop_equiv preamble.g
-//       (comp_pre preamble.c)
-//       (Tm_Star (list_as_vprop p.unmatched) p.matched) =
-//       p.veq in
-//     // use veq_unm
-//     let veq : vprop_equiv preamble.g
-//       (comp_pre preamble.c)
-//       (Tm_Star (Tm_Star unm (list_as_vprop unmatched)) p.matched) = magic () in
-//     // stars rearrangement
-//     let veq : vprop_equiv preamble.g
-//       (comp_pre preamble.c)
-//       (Tm_Star (list_as_vprop unmatched) matched) = magic () in
-//     /////
-
-//     Some { p with
-//            matched;
-//            unmatched;
-//            remaining;
-//            steps = p.steps;
-//            ss;
-//            remaining_typing = magic ();  // remaining and matched are sub vprops of original ones,
-//                                          // whose typing came in with the orignal prover state
-//            unmatched_typing = magic ();
-//            steps_typing;
-//            veq;
-//            props = (); }
-  
-//   | _ -> admit ()
-
-// module RT = FStar.Reflection.Typing
-
-// val subset_bool (#a:eqtype) (s1 s2:Set.set a)
-//   : Tot (b:bool { b ==> Set.subset s1 s2 })
-
-// #push-options "--z3rlimit_factor 4 --ifuel 1 --fuel 1"
-// let intro_exists_sub_prover_state (#preamble:_) (p:prover_state preamble)
-//   (u:universe) (t:term) (body:vprop)
-//   (unmatched':list vprop)
-//   (_:squash (p.unmatched == (Tm_ExistsSL u (null_binder t) body)::unmatched'))
-//   (y:var {y == fresh preamble.g})
-//   : preamble_sub:prover_state_preamble &
-//     prover_state preamble_sub =
-  
-//   let g' = push_binding preamble.g y t in
-//   assume (g' `env_extends` preamble.g);
-
-//   //// create a sub prover preamble ////
-//   let g0_sub = preamble.g0 in
-//   let g_sub = g' in
-//   let ctxt_sub = list_as_vprop p.remaining in
-//   let ctxt_typing_sub : vprop_typing g0_sub (list_as_vprop p.remaining) =
-//     p.remaining_typing in
-//   let witness_tm = tm_var {
-//     nm_index = y;
-//     nm_ppname = ppname_default;
-//   } in
-//   // what should erased be?
-//   let t_sub = wr (Tm_IntroExists {
-//     erased = false;
-//     p = Tm_ExistsSL u (null_binder t) body;
-//     witnesses = [witness_tm];
-//     should_check = should_check_true
-//   }) in
-//   let c_sub = comp_intro_exists u (null_binder t) body witness_tm in
-//   // the t and Tm_ExistsSL should come from typing of matched
-//   // and some inversions
-//   let t_typing_sub : st_typing g' t_sub c_sub =
-//     T_IntroExists g' u (null_binder t) body witness_tm
-//       (magic ())  // typing of t
-//       (magic ())  // typing of Tm_ExistsSL
-//       (magic ())  // typing of witness_tm
-//   in
-
-//   let uvs_sub = Map.upd preamble.uvs y t in
-//   assume (~ (Map.contains preamble.uvs y));
-//   assume (dom_env g_sub == Set.union (dom_env preamble.g) (Set.singleton y));
-//   assume (~ (Set.mem y (dom_env preamble.g0)));
-//   assume (forall (x:var). Map.contains uvs_sub x ==>
-//                           env_contains g_sub x (Map.sel uvs_sub x));
-
-//   let preamble_sub = {
-//     g0 = g0_sub;
-//     g = g_sub;
-//     ctxt = ctxt_sub;
-//     ctxt_typing = ctxt_typing_sub;
-//     t = t_sub;
-//     c = c_sub;
-//     t_typing = t_typing_sub;
-
-//     uvs = uvs_sub;
-//     uvs_props = ()
-//   } in
-//   /////
-  
-//   // create a sub prover state /////
-//   let matched_sub = Tm_Emp in
-//   let unmatched_sub = vprop_as_list (comp_pre preamble_sub.c) in
-//   let remaining_sub = p.remaining in
-
-//   let remaining_typing:vprop_typing preamble_sub.g0 (list_as_vprop remaining_sub) =
-//     p.remaining_typing in
-
-//   // get from inversion of t_typing_sub
-//   let unmatched_typing:vprop_typing preamble_sub.g (list_as_vprop unmatched_sub) =
-//     magic () in
-  
-//   let (| steps_sub, steps_typing_sub |) = idem_steps preamble_sub.g0 preamble_sub.ctxt in
-//   assume (apply_ss p.ss Tm_Emp == Tm_Emp);
-//   assume (list_as_vprop (vprop_as_list preamble_sub.ctxt) == preamble_sub.ctxt);
-//   let steps_typing_sub : st_typing preamble_sub.g0 steps_sub
-//     (ghost_comp preamble_sub.ctxt
-//        (Tm_Star (list_as_vprop remaining_sub) Tm_Emp)) = coerce_eq steps_typing_sub () in
-
-//   // matched_sub is emp, and list_as_vprop and vprop_as_list should cancel
-//   let veq_sub : vprop_equiv preamble_sub.g
-//     (comp_pre preamble_sub.c)
-//     (Tm_Star (list_as_vprop unmatched_sub) matched_sub) = magic () in
-
-//   let ss_sub = p.ss in
-
-//   assume (apply_ss ss_sub matched_sub == Tm_Emp);
-
-//   let prover_state_sub : prover_state preamble_sub = {
-//     matched = matched_sub;
-//     unmatched = unmatched_sub;
-//     remaining = remaining_sub;
-//     steps = steps_sub;
-//     ss = ss_sub;
-//     remaining_typing;
-//     unmatched_typing;
-//     steps_typing = steps_typing_sub;
-//     veq = veq_sub;
-//     props = ();
-//   } in
-
-//   (| preamble_sub, prover_state_sub |)
-
-
-
-// let intro_exists_step (#preamble:_) (p:prover_state preamble)
-//   (u:universe) (t:term) (body:vprop)
-//   (unmatched':list vprop)
-//   (_:squash (p.unmatched == (Tm_ExistsSL u (null_binder t) body)::unmatched'))
-//   (prover:(#(preamble:_) ->
-//            p:prover_state preamble ->
-//            T.Tac (option (p':prover_state preamble { p'.unmatched == [] /\
-//                                                      p'.ss `ss_extends` p.ss }))))
-
-//   : T.Tac (option (p':prover_state preamble { p'.ss `ss_extends` p.ss })) =
-  
-//   let y = fresh preamble.g in
-//   let (| preamble_sub, prover_state_sub |) =
-//     intro_exists_sub_prover_state p u t body unmatched' () y in
-//   let t_sub = preamble_sub.t in
-//   let c_sub = preamble_sub.c in
-//   let t_typing_sub = preamble_sub.t_typing in
-
-//   let popt = prover prover_state_sub in
-//   match popt with
-//   | None -> None
-//   | Some psub ->
-//     // make sure witness is solved, and exists is uvars free
-//     if Set.mem y (Map.domain psub.ss) &&
-//        subset_bool (uvars (Tm_ExistsSL u (null_binder t) body) preamble_sub.uvs) (Map.domain psub.ss)
-//     then begin
-//       let steps_typing_sub : st_typing preamble_sub.g0 psub.steps
-//         (ghost_comp
-//            (list_as_vprop p.remaining)
-//            (Tm_Star (list_as_vprop psub.remaining) (apply_ss psub.ss psub.matched))) = psub.steps_typing in
+                  (ghost_comp
+                     preamble.ctxt (Tm_Star remaining_ctxt (Tm_Star (Psubst.subst_term sp.ss (Tm_ExistsSL u b body)) p.solved_goals))) = magic () in
       
-//       let veq_sub : vprop_equiv preamble_sub.g
-//         (comp_pre c_sub)
-//         (Tm_Star (list_as_vprop []) psub.matched) = psub.veq in
-//       // some manipulation of veq_sub
-//       let veq_sub : vprop_equiv preamble_sub.g (comp_pre c_sub) psub.matched = magic () in
-//       let veq_sub : vprop_equiv preamble_sub.g
-//         (apply_ss psub.ss (comp_pre c_sub))
-//         (apply_ss psub.ss psub.matched) =
-//         veq_ss preamble_sub.g0 preamble_sub.uvs veq_sub psub.ss in
+      assume (Psubst.subst_term sp.ss (Tm_ExistsSL u b body) ==
+              Psubst.subst_term sp_ss (Tm_ExistsSL u b body));  // sp_ss = sp.ss - x, and x is not free in Tm_ExistsSL
+       
+      let steps_typing:
+        st_typing (pst_env preamble.uvs ss_new)
+                  steps
+                  (ghost_comp
+                     preamble.ctxt (Tm_Star remaining_ctxt (Tm_Star (Psubst.subst_term sp_ss (Tm_ExistsSL u b body)) p.solved_goals))) =
+        coerce_eq steps_typing () in
 
-//       // THIS IS TODO, BUT WE SHOULD BE ABLE TO STRENGTHEN veq_sub to preamble_sub.g0
-//       // Need a lemma that says, if freevars t in g, and no uvars in t, then freevars t in g0
-//       //   Then we can use strengthening lemmas
-//       let veq_sub : vprop_equiv preamble_sub.g0
-//         (apply_ss psub.ss (comp_pre c_sub))
-//         (apply_ss psub.ss psub.matched) = magic () in
+      let c_pre_inv:
+        vprop_equiv (pst_env preamble.uvs p.ss)
+                    (Psubst.subst_term p.ss (comp_pre preamble.c))
+                    (Tm_Star (list_as_vprop p.unsolved_goals) p.solved_goals) = p.c_pre_inv in
 
-//       // use veq_sub on steps_typing_sub
-//       let steps_typing_sub : st_typing preamble_sub.g0 psub.steps
-//         (ghost_comp
-//            (list_as_vprop p.remaining)
-//            (Tm_Star (list_as_vprop psub.remaining) (apply_ss psub.ss (comp_pre c_sub)))) = magic () in
+      let (| _, c_pre_inv |) = apply_partial_subs_veq uvs sp_ss c_pre_inv in
+      assert (Psubst.subst_term sp_ss (Psubst.subst_term p.ss (comp_pre preamble.c)) ==
+              Psubst.subst_term (Psubst.push p.ss sp_ss) (comp_pre preamble.c));
+      let c_pre_inv:
+        vprop_equiv (pst_env preamble.uvs ss_new)
+                    (Psubst.subst_term (Psubst.push p.ss sp_ss) (comp_pre preamble.c))
+                    (Psubst.subst_term sp_ss (Tm_Star (list_as_vprop ((Tm_ExistsSL u b body)::unsolved_goals')) p.solved_goals)) =
+        coerce_eq c_pre_inv () in
+      let c_pre_inv:
+        vprop_equiv (pst_env preamble.uvs ss_new)
+                    (Psubst.subst_term (Psubst.push p.ss sp_ss) (comp_pre preamble.c))
+                    (Tm_Star (Psubst.subst_term sp_ss (list_as_vprop unsolved_goals')) (Tm_Star (Psubst.subst_term sp_ss (Tm_ExistsSL u b body)) p.solved_goals))
+        = magic () in  // some rearrangement in the above c_pre_inv
 
-//       let t_typing_sub : st_typing preamble_sub.g t_sub c_sub = t_typing_sub in
-//       assert (comp_post c_sub == Tm_ExistsSL u (null_binder t) body);
+      
+      // move t_typing from p over
+      let t_typing:
+        st_typing (pst_env preamble.uvs p.ss)
+                  (Psubst.subst_st_term p.ss preamble.t)
+                  (Psubst.subst_comp p.ss preamble.c) = p.t_typing in
+      
+      let (| _, t_typing |) = apply_partial_subs uvs sp_ss t_typing in
+      let t_typing:
+        st_typing (pst_env preamble.uvs ss_new)
+                  (Psubst.subst_st_term ss_new preamble.t)
+                  (Psubst.subst_comp ss_new preamble.c) = coerce_eq t_typing () in
 
-//       let t_typing_sub : st_typing preamble_sub.g
-//         (apply_ss_st psub.ss t_sub)
-//         (apply_c psub.ss c_sub) = typing_ss preamble_sub.g0 preamble_sub.uvs t_typing_sub psub.ss in
 
-//       // AGAIN WE NEED A STRENGTHENING STEP HERE TO TAKE t_typing_sub to preamble_sub.g0
-//       // Need a lemma that says, if freevars t in g, and no uvars in t, then freevars t in g0
-//       //   Then we can use strengthening lemmas
-//       let t_typing_sub : st_typing preamble_sub.g0
-//         (apply_ss_st psub.ss t_sub)
-//         (apply_c psub.ss c_sub) = magic () in
+      let ss = ss_new in
+      let solved_goals = Tm_Star (Psubst.subst_term sp_ss (Tm_ExistsSL u b body)) p.solved_goals in
+      let unsolved_goals = vprop_as_list (Psubst.subst_term sp_ss (list_as_vprop unsolved_goals')) in
+      let remaining_ctxt = vprop_as_list remaining_ctxt in
+      let steps = steps in
 
-//       // assume (stateful_comp (apply_c psub.ss c_sub));
-//       // assume (comp_pre (apply_c psub.ss c_sub) == apply_ss psub.ss (comp_pre c_sub));
-//       // assume (comp_post (apply_c psub.ss c_sub) == apply_ss psub.ss (comp_post c_sub));
+      let t_typing
+        : st_typing (pst_env preamble.uvs ss)
+                    (Psubst.subst_st_term ss preamble.t)
+                    (Psubst.subst_comp ss preamble.c) = t_typing in
 
-//       // g0 |- { p.remaining } psub.steps { psub.remaining * apply_ss psub.ss (comp_pre c_sub) }
-//       // g0 |- { apply_ss psub.ss (comp_pre c_sub) } apply_ss_st psub.ss t_sub { apply_ss psub.ss (comp_post c_sub) }
-//       // so we can bind these ... and note that c_sub is also ghost
-//       let steps : st_term = magic () in  // Tm_Bind steps (apply_ss_st psub.ss t_sub)
-//       let steps_c = ghost_comp (list_as_vprop p.remaining)
-//                                (Tm_Star (list_as_vprop psub.remaining)
-//                                         (apply_ss psub.ss (Tm_ExistsSL u (null_binder t) body))) in
-//       let steps_typing : st_typing preamble_sub.g0 steps steps_c = magic () in  // bind typing
-//       let steps_typing : st_typing preamble.g0 steps steps_c = steps_typing in
+      let remaining_ctxt_typing:
+        vprop_typing g0 (list_as_vprop remaining_ctxt) = sp.remaining_ctxt_typing in
 
-//       let psteps_typing : st_typing preamble.g0 p.steps
-//         (ghost_comp preamble.ctxt
-//                     (Tm_Star (list_as_vprop p.remaining)
-//                              (apply_ss p.ss p.matched))) = p.steps_typing in
+      let steps_typing
+        : st_typing (pst_env preamble.uvs ss)
+                    steps
+                    (ghost_comp
+                       preamble.ctxt
+                       (Tm_Star (list_as_vprop remaining_ctxt) solved_goals)) = steps_typing in
 
-//       let ss_new = Map.restrict (Map.domain preamble.uvs) psub.ss in
-//       assume (~ (Map.contains preamble.uvs y));
-//       assume (~ (Map.contains p.ss y));
-//       assert (ss_new `ss_extends` p.ss);
-//       assert (well_typed_substitution preamble.g0 preamble.uvs ss_new);
 
-//       extends_apply preamble.g0 preamble.uvs ss_new p.ss p.matched;
+      Some ({
+        ss; solved_goals; unsolved_goals; remaining_ctxt; steps;
+        t_typing; unsolved_goals_typing = magic (); remaining_ctxt_typing; steps_typing;
+        c_pre_inv = magic (); solved_goals_closed = magic ()  // we need to add a runtime check that Tm_ExistsSL u t body is fully closed
+      })
+    end
+    else None
 
-//       let psteps_typing : st_typing preamble.g0 p.steps
-//         (ghost_comp preamble.ctxt
-//                     (Tm_Star (list_as_vprop p.remaining)
-//                              (apply_ss ss_new p.matched))) = coerce_eq psteps_typing () in
-
-//       // ss_new = psub.ss - y, and y does not occur free in Tm_ExistsSL u t body
-//       assume (apply_ss psub.ss (Tm_ExistsSL u (null_binder t) body) ==
-//               apply_ss ss_new (Tm_ExistsSL u (null_binder t) body));
-//       let steps_typing : st_typing preamble.g0 steps
-//         (ghost_comp (list_as_vprop p.remaining)
-//                     (Tm_Star (list_as_vprop psub.remaining)
-//                              (apply_ss ss_new (Tm_ExistsSL u (null_binder t) body)))) = steps_typing in
-
-//       // g0 |- { preamble.ctxt } p.steps { p.remaining * apply_ss ss_new p.matched }
-//       // g0 |- { p.remaining } steps { psub.remaining * apply_ss ss_new (Tm_ExistsSL u t body) }
-//       //
-//       // bind them
-//       let steps_new : st_term = magic () in
-//       let steps_typing_new : st_typing preamble.g0 steps_new
-//         (ghost_comp preamble.ctxt
-//                     (Tm_Star (list_as_vprop psub.remaining)
-//                              (apply_ss ss_new (Tm_Star (Tm_ExistsSL u (null_binder t) body) p.matched)))) =
-//         magic () in
-
-//       let matched_new = Tm_Star (Tm_ExistsSL u (null_binder t) body) p.matched in
-//       let unmatched_new = unmatched' in
-//       let remaining_new = psub.remaining in
-//       let steps_new = steps_new in
-//       let ss_new = ss_new in
-
-//       let remaining_typing_new : vprop_typing preamble.g0 (list_as_vprop remaining_new) =
-//         psub.remaining_typing in
-
-//       // unmatched' is the left component of star term,
-//       // whose typing came in to us
-//       let unmatched_typing : vprop_typing preamble.g (list_as_vprop unmatched') = magic () in
-
-//       let steps_typing_new : st_typing preamble.g0 steps_new
-//         (ghost_comp preamble.ctxt
-//                     (Tm_Star (list_as_vprop remaining_new)
-//                              (apply_ss ss_new matched_new))) = steps_typing_new in
-
-//       // move Tm_ExistsSL from unmatched to matched
-//       let veq : vprop_equiv preamble.g (comp_pre preamble.c)
-//                                        (Tm_Star (list_as_vprop unmatched_new) matched_new) = magic () in
-
-//       assert (well_typed_substitution preamble.g0 preamble.uvs ss_new);
-//       assert (uvars matched_new preamble.uvs `Set.subset` Map.domain ss_new);
-
-//       Some {
-//         matched = matched_new;
-//         unmatched = unmatched_new;
-//         remaining = remaining_new;
-//         steps = steps_new;
-//         ss = ss_new;
-//         remaining_typing = remaining_typing_new;
-//         unmatched_typing;
-//         steps_typing = steps_typing_new;
-//         veq;
-//         props = ();
-//       }
-//     end
-//     else None
-// #pop-options
-
-// // let has_no_uvars_from (t:term) (uvs:Set.set var) =
-// //   freevars t `Set.disjoint` uvs
-
-// // type uv_st =
-// //   uvs:Set.set var & Map.t var (t:term { t `has_no_uvars_from` uvs})
-
-// // let subst_uvs (t:term) (uvs:uv_st) : term = admit ()
-// // let subst_uvs_st_term (t:st_term) (uvs:uv_st) : st_term = admit ()
-
-// // noeq
-// // type prover_state (g:env) (preamble:prover_state_preamble g) = {
-// //   (* uvars and their solutions *)
-// //   uv_st : uv_st;
-
-// //   (* the in-progress proof state *)
-// //   matched_pre:term; (* conjuncts that we have already derived *)
-// //   unmatched_pre:list term; (* conjuncts remaining to be derived *)
-// //   remaining_ctxt:list term; (* unused conjuncts in the context *)
-
-// //   (* Ghost proof steps witnessing the derivation of matched_pre from ctxt *)
-// //   proof_steps : st_term;
-
-// //   ctxt_no_uvs : squash (
-// //     preamble.ctxt `has_no_uvars_from` (dfst uv_st) /\
-// //     list_as_vprop remaining_ctxt `has_no_uvars_from` (dfst uv_st)
-// //   );
-
-// //   proof_steps_typing:
-// //     st_typing g
-// //       (subst_uvs_st_term proof_steps uv_st)
-// //       (ghost_comp preamble.ctxt (Tm_Star (subst_uvs (list_as_vprop remaining_ctxt) uv_st)
-// //                                          (subst_uvs matched_pre uv_st)));
-
-// //   pre_equiv:
-// //     vprop_equiv g
-// //       (subst_uvs (comp_pre preamble.c) uv_st)
-// //       (Tm_Star (subst_uvs (list_as_vprop unmatched_pre) uv_st) (subst_uvs matched_pre uv_st));
-// // }
-
-// // let proof_steps_post (#g:_) (#preamble:_) (p:prover_state g preamble) : vprop =
-// //   Tm_Star (list_as_vprop p.remaining_ctxt) (subst_uvs p.matched_pre p.uv_st)
-
-// // let bind_proof_steps_with (#g:env) (#preamble:_) (p:prover_state g preamble)
-// //   (t:st_term)
-// //   (c:comp_st {comp_pre c == proof_steps_post p})
-// //   (t_typing:st_typing g t c)
-// //   : (t':st_term & st_typing g t' (comp_st_with_pre c preamble.ctxt))
-// //   = admit()
-
-// // type prover_step_t =
-// //   #g:_ ->
-// //   #preamble:_ ->
-// //   p:prover_state g preamble ->
-// //   T.Tac (option (prover_state g preamble))
-
-// // //
-// // // result of an intro (pure, exists, rewrite) step
-// // //   that consumes some vprop v from p.unmatched_pre
-// // //
-
-// // let intro_comp (c:comp) =
-// //   C_STGhost? c /\ comp_u c == u_zero /\ comp_res c == tm_unit
-
-// // //
-// // // A proof step that provides v, eating away some of the ctxt
-// // //
-// // noeq
-// // type proof_step (g:env) (ctxt:list vprop) (v:vprop) = {
-// //   remaining' : list vprop;
-
-// //   t' : st_term;
-// //   c' : c:comp { intro_comp c /\ comp_post c == v };
-// //   t'_typing : st_typing g t' c';
-
-// //   remaining_equiv : vprop_equiv g (list_as_vprop ctxt)
-// //                                   (Tm_Star (comp_pre c') (list_as_vprop remaining'));
-// // }
-
-// // // An intro step that makes progress by solving one conjunct
-// // // v from the p.unmatched_pre
-// // noeq
-// // type intro_from_unmatched_step (#g:env) (#preamble:_) (p:prover_state g preamble) = {
-// //   uv_st : uv_st;
-
-// //   v : vprop;
-
-// //   // new unmatched pre and remaining ctxt
-// //   remaining' : list vprop; 
-// //   unmatched' : list vprop;
-
-// //   t' : st_term;
-// //   c' : c:comp { intro_comp c /\ comp_post c == v };
-// //   t'_typing : st_typing g t' c';
- 
-// //   // relation between new and old unmatched_pre and remaining_ctxt
-// //   unmatched_equiv : vprop_equiv g (list_as_vprop p.unmatched_pre)
-// //                                   (Tm_Star v (list_as_vprop unmatched'));
-// // }
-
-// // type proof_step_fn =
-// //   #g:_ ->
-// //   #ctxt:_ ->
-// //   #v:vprop ->
-// //   tot_typing g (list_as_vprop ctxt) Tm_VProp ->
-// //   tot_typing g v Tm_VProp ->
-// //   T.Tac (option (proof_step g ctxt v))
-
-// // type intro_from_unmatched_fn =
-// //   #g:_ ->
-// //   #preamble:_ ->
-// //   p:prover_state g preamble ->
-// //   T.Tac (option (intro_from_unmatched_step p))
-
-// // val apply_proof_step
-// //   (#g:env)
-// //   (#preamble:_)
-// //   (p:prover_state g preamble)
-// //   (v:vprop)
-// //   (r:proof_step g p.remaining_ctxt v)  
-// //   : T.Tac (p':prover_state g preamble {
-// //       p'.matched_pre == p.matched_pre /\
-// //       p'.unmatched_pre == p.unmatched_pre /\
-// //       p'.remaining_ctxt == v::r.remaining'
-// //     })
-
-// // val apply_intro_from_unmatched_step
-// //   (#g:env)
-// //   (#preamble:_)
-// //   (#p:prover_state g preamble)
-// //   (r:intro_from_unmatched_step p)
-// //   : T.Tac (p':prover_state g preamble {
-// //       p'.matched_pre == Tm_Star p.matched_pre r.v /\
-// //       p'.unmatched_pre == r.unmatched' /\
-// //       p'.remaining_ctxt == r.ps.remaining'
-// //     })
